data_structure/spatial_graph_VST.v
@@ -1,20 +1,10 @@
+Require Import RamifyCoq.veric_ext.SeparationLogic.
 Require Import RamifyCoq.data_structure.spatial_graph.
 Require Import RamifyCoq.msl_ext.abs_addr.
 Require Import RamifyCoq.msl_ext.seplog.
 Require Import VST.veric.SeparationLogic.
 Require Import RamifyCoq.msl_ext.alg_seplog.
-Require Import RamifyCoq.veric_ext.SeparationLogic.
 Require Import RamifyCoq.sample_mark.env_mark.
-
-(* Move into VST *)
-Lemma block_eq_dec: forall b1 b2: block, {b1 = b2} + {b1 <> b2}.
-Proof. exact (Coqlib.peq). Qed.
-
-Lemma PV_eq_dec: forall x y: pointer_val, {x = y} + {x <> y}.
-Proof.
-  intros; destruct x, y; [| right | right | left]; try congruence.
-  destruct (block_eq_dec b b0), (Int.eq_dec i i0); [left | right | right | right]; congruence.
-Qed.
 
 (* Move into env_mark. *)
 Definition node_type := (talignas 4%N (Tstruct _Node noattr)).
